primitive_laws.v
@@ -1,13 +1,14 @@
-From iris.program_logic Require Export ectx_lifting weakestpre.
+From iris.program_logic Require Export ectx_lifting total_ectx_lifting weakestpre.
 From iris.proofmode Require Import tactics.
 From chanlang Require Import lang notation network_ra.
 From iris Require Import options.
+From iris.base_logic.lib Require Import invariants.
 
 (* Ghost state for reasoning about chan_lang threadpool. *)
 Class chanG Σ :=
   ChanG {
       chan_invG : invG Σ;
-      chan_gen_networkG :> gen_networkGS chan_id (option (gset val)) Σ;
+      chan_gen_networkG :> gen_networkGS loc (option (gset val)) Σ;
     }.
 
 Global Instance chan_irisG `{!chanG Σ} : irisG chan_lang Σ :=
@@ -18,3 +19,61 @@ Global Instance chan_irisG `{!chanG Σ} : irisG chan_lang Σ :=
   num_laters_per_step _ := 0;
   state_interp_mono _ _ _ _ := fupd_intro _ _
 }.
+
+Ltac inv_head_step :=
+  repeat match goal with
+  | _ => progress simplify_map_eq/= (* simplify memory stuff *)
+  | H : to_val _ = Some _ |- _ => apply of_to_val in H
+  | H : head_step ?e _ _ _ _ _ |- _ =>
+     try (is_var e; fail 1); (* inversion yields many goals if [e] is a variable
+     and should thus better be avoided. *)
+     inversion H; subst; clear H
+  end.
+
+Create HintDb head_step.
+Global Hint Extern 0 (head_reducible _ _) => eexists _, _, _, _; simpl : head_step.
+
+(* [simpl apply] is too stupid, so we need extern hints here. *)
+Global Hint Extern 1 (head_step _ _ _ _ _ _) => econstructor : head_step.
+Global Hint Extern 0 (head_step NewCh _ _ _ _ _) => apply alloc_newch : head_step.
+
+Section proof.
+  Context `{!chanG Σ}.
+
+  Notation iProp := (iProp Σ).
+
+  Definition true : iProp := ⌜ True ⌝.
+
+  Definition wp_newch :
+    {{{ true }}} newch {{{ l, RET LitV (LitLoc l); l ↦ Some ∅ }}}.
+  Proof.
+    iIntros (Φ) "Pre Post".
+    iApply wp_lift_atomic_head_step; [done|].
+    iIntros (σ1 ns κ κs nt) "Hσ !>"; iSplit; first by auto with head_step.
+    iIntros "!>" (v2 σ2 efs Hstep); inv_head_step.
+    iMod (gen_network_alloc σ1.(chan) c empty with "Hσ") as "[Hσ Hl]"; first done.
+    iModIntro. iFrame. iApply "Post".
+    iApply "Hl".
+  Qed.
+
+  Definition threadpool := gmap loc (option (gset val)).
+
+  (* Definition recv_inv v (P : iProp) (Q : threadpool -> chan_lang.val -> iProp) : iProp := *)
+  (*   (P ∗ ⌜v = NONE⌝ ∨ ∃ M m, Q M m ∗ ⌜v = SOMEV m⌝)%I. *)
+
+  (* Definition is_recv P Q v := *)
+  (*   inv N (recv_inv v P Q). *)
+
+  (* (* Section 7.2 Proof of blocking receive (10) *) *)
+  (* Lemma wp_tryrecv P (Q : threadpool -> chan_lang.val -> iProp) c : *)
+  (*   {{{ P }}} tryrecv c {{{ v , RET v; is_recv P Q v }}}. *)
+  (* Proof. *)
+  (*   iIntros (Φ) "P Q". *)
+  (*   iApply wp_lift_atomic_head_step; [done|]. *)
+  (*   iIntros (σ1 ns κ κs nt) "Hσ !>". iSplit. *)
+  (*   (* - first by euto with head_step. iMod "Q (tryrecv c)". *) *)
+  (*   (*   unfold head_reducible. iExists _, _, _, _. iSimpl. *) *)
+  (*   (*   iMod "Q".  as  "_". *) *)
+  (* Admitted. *)
+
+End proof.
